added rounds relation

Grandpa/src/OpaqueRound.v
@@ -4,6 +4,8 @@ Require Import Voters.
 Require Import Round.
 Require Import Estimate.
 
+Require Import Coq.Program.Equality.
+
 Export Round.
 
 Require Import Message.
@@ -13,96 +15,132 @@ Require Import Classes.Math.All.
 (** *OpaqueRoundState
 This didn't exist in the paper, is a convenient newtype around [RoundState].
 
-The [OpaqueRoundState] type allow us to store different rounds in a single 
+The [OpaqueRoundState] type allow us to store different rounds in a single
 collection like a [vector] or a [list].
 
-Another advantage is that we don't need to explicitly pass around the 
+Another advantage is that we don't need to explicitly pass around the
 parameters of a round.
 *)
 
-Variant OpaqueRoundState: Type := 
+Variant OpaqueRoundState: Type :=
   | OpaqueRoundStateC {total_voters round_number}
     {prevote_voters:Voters}
     {precommit_voters: Voters}
     {round_start_time:Time}
     {time:Time}
-    (round_state: 
-      RoundState 
-        total_voters 
-        prevote_voters 
-        precommit_voters 
-        round_start_time 
-        round_number 
-        time 
+    (round_state:
+      RoundState
+        total_voters
+        prevote_voters
+        precommit_voters
+  round_start_time
+        round_number
+        time
     ).
 
 Definition get_prevote_voters (o:OpaqueRoundState) : Voters
   :=
-  match o with 
-  | OpaqueRoundStateC r => Round.get_prevote_voters r 
+  match o with
+  | OpaqueRoundStateC r => Round.get_prevote_voters r
   end.
 
 Definition get_precommit_voters (o:OpaqueRoundState) : Voters
   :=
-  match o with 
-  | OpaqueRoundStateC r => Round.get_precommit_voters r 
+  match o with
+  | OpaqueRoundStateC r => Round.get_precommit_voters r
   end.
 
 Definition get_start_time (o:OpaqueRoundState) : Time
   :=
-  match o with 
-  | OpaqueRoundStateC r => Round.get_start_time r 
+  match o with
+  | OpaqueRoundStateC r => Round.get_start_time r
+  end.
+
+Definition get_time_increment (o:OpaqueRoundState) : Time
+  :=
+  match o with
+  | OpaqueRoundStateC r => Round.get_time_increment r
   end.
 
 Definition get_round_number (o:OpaqueRoundState) : RoundNumber
   :=
-  match o with 
+  match o with
   | OpaqueRoundStateC r => Round.get_round_number r
   end.
 
 Definition get_total_voters (o:OpaqueRoundState) : nat
   :=
-  match o with 
-  | OpaqueRoundStateC r => Round.get_total_voters r 
+  match o with
+  | OpaqueRoundStateC r => Round.get_total_voters r
   end.
 
 Definition get_all_prevote_votes (o:OpaqueRoundState) : (Votes (get_prevote_voters o))
   :=
-  match o with 
-  | OpaqueRoundStateC r => Round.get_prevote_votes r 
+  match o with
+  | OpaqueRoundStateC r => Round.get_prevote_votes r
   end.
 
 Definition get_all_precommit_votes (o:OpaqueRoundState) : (Votes (get_precommit_voters o))
   :=
-  match o with 
-  | OpaqueRoundStateC r => Round.get_precommit_votes r 
+  match o with
+  | OpaqueRoundStateC r => Round.get_precommit_votes r
   end.
 
-Definition is_completable (o:OpaqueRoundState) 
+Definition is_completable (o:OpaqueRoundState)
   : bool
   :=
-  match o with 
-  | OpaqueRoundStateC r => Estimate.is_completable r 
+  match o with
+  | OpaqueRoundStateC r => Estimate.is_completable r
   end.
 
-Definition get_estimate (o:OpaqueRoundState) 
+Definition get_estimate (o:OpaqueRoundState)
   : option AnyBlock
   :=
-  match o with 
-  | OpaqueRoundStateC r => Estimate.get_estimate r 
+  match o with
+  | OpaqueRoundStateC r => Estimate.get_estimate r
   end.
 
 
 Open Scope math.
 Open Scope natWrapper.
 
+Program Definition update_opaque_round_state
+  (o:OpaqueRoundState)
+  (time_increment:Time)
+  (new_prevotes: Votes (get_prevote_voters o))
+  (new_precommits:Votes (get_precommit_voters o))
+  : OpaqueRoundState
+  :=
+  match o with
+  | @OpaqueRoundStateC
+      total_voters
+      round_number
+      prevote_voters
+      precommit_voters
+      start_time
+      time
+      r =>
+        OpaqueRoundStateC(
+          Round.RoundStateUpdate
+          total_voters
+          prevote_voters
+          precommit_voters
+          start_time
+          round_number
+          r
+          time_increment
+          new_prevotes
+          new_precommits
+        )
+  end.
+
 (**
 It add the precommit or prevote vote represented
 by a message to the particular round it is related to.
 
-If the message came from a voter outside of the set of 
-precommiters or prevoters for the round, we ignore the vote. 
-In the paper they assumed that every participant is capable 
+If the message came from a voter outside of the set of
+precommiters or prevoters for the round, we ignore the vote.
+In the paper they assumed that every participant is capable
 to determine the round participants.
 
 If the message isn't a precommit or prevote we do nothing.
@@ -114,53 +152,131 @@ Definition update_votes_with_msg
   :=
   match opaque with
   | OpaqueRoundStateC r =>
-    let bizantiners_number := Round.get_total_voters r
+    let new_time_increment : Time := (msg.(Message.time) - (get_start_time opaque + get_time_increment opaque))
     in
-    let prevote_voters := Round.get_prevote_voters r
-    in
-    let precommit_voters := Round.get_precommit_voters r
-    in
-    let start_time := Round.get_start_time r
-    in
-    let old_increment := Round.get_start_time r
-    in
-    let round_number := Round.get_round_number r
-    in
-    let new_time_increment : Time := (msg.(Message.time) - (start_time + old_increment))
-    in
-    match Message.message_to_prevote_vote msg prevote_voters with
-    | Some new_votes => 
-       OpaqueRoundStateC (
-         RoundStateUpdate 
-           bizantiners_number
-           prevote_voters 
-           precommit_voters 
-           start_time 
-           round_number 
-           r 
-           new_time_increment 
-           (VotesC prevote_voters (List.cons new_votes List.nil))
-           (VotesC precommit_voters List.nil) 
-         )
-    | _ => 
-      match Message.message_to_precommit_vote msg precommit_voters with
-      | Some new_votes => 
-         OpaqueRoundStateC (
-           RoundStateUpdate 
-             bizantiners_number
-             prevote_voters 
-             precommit_voters 
-             start_time 
-             round_number 
-             r 
-             new_time_increment 
-             (VotesC prevote_voters List.nil) 
-             (VotesC precommit_voters (List.cons new_votes List.nil))
-           )
+    match Message.message_to_prevote_vote msg (get_prevote_voters opaque)with
+    | Some new_votes =>
+        update_opaque_round_state opaque new_time_increment
+           (VotesC (get_prevote_voters opaque) (List.cons new_votes List.nil))
+           (VotesC (get_precommit_voters opaque) List.nil)
+    | _ =>
+      match Message.message_to_precommit_vote msg (get_precommit_voters opaque) with
+      | Some new_votes =>
+        update_opaque_round_state opaque new_time_increment
+             (VotesC (get_prevote_voters opaque) List.nil)
+             (VotesC (get_precommit_voters opaque) (List.cons new_votes List.nil))
       | _ => opaque
       end
      end
   end.
+
+
+Section IsUpdateRelation.
+
+Inductive IsUpdateOf : OpaqueRoundState -> OpaqueRoundState -> Prop
+  :=
+  | SameRoundState o : IsUpdateOf o o
+  | IsRoundUpdate o1 o2 (is_related : IsUpdateOf o1 o2)
+      (time_increment:Time)
+      (new_prevotes: Votes (get_prevote_voters o2))
+      (new_precommits:Votes (get_precommit_voters o2))
+      : IsUpdateOf o1 (update_opaque_round_state o2 time_increment new_prevotes new_precommits).
+
+
+Lemma is_update_reflexivity o : IsUpdateOf o o.
+Proof.
+  apply SameRoundState.
+Qed.
+
+Lemma origin_isnt_update_of_not_origin
+    {total_voters round_number}
+    {prevote_voters:Voters}
+    {precommit_voters: Voters}
+    {round_start_time:Time}
+    {time:Time}
+    o
+      (time_increment:Time)
+      (new_prevotes: Votes (get_prevote_voters o))
+      (new_precommits:Votes (get_precommit_voters o))
+    : IsUpdateOf (update_opaque_round_state o time_increment new_prevotes new_precommits) (OpaqueRoundStateC (InitialRoundState total_voters prevote_voters precommit_voters round_start_time round_number)) -> False.
+Proof.
+  intro H.
+  destruct o.
+  inversion H.
+  destruct o2.
+  inversion H2.
+Qed.
+
+
+Lemma is_update_of_previous o1 o2 :
+  forall ti npv npr,
+  IsUpdateOf (update_opaque_round_state o1 ti npv npr) o2
+  -> IsUpdateOf o1 o2.
+Proof.
+  destruct o2.
+  intros *.
+  intro H.
+  Opaque update_opaque_round_state.
+  induction round_state.
+  - destruct o1.
+    exfalso. eapply origin_isnt_update_of_not_origin. eauto.
+  Admitted.
+
+
+Lemma is_update_transitive {o1} o2
+  : IsUpdateOf o1 o2
+  -> (forall {o3}, IsUpdateOf o2 o3
+    -> IsUpdateOf o1 o3).
+Proof.
+  intro H.
+  induction H.
+  - auto.
+  - intros o3 H2.
+    apply IHIsUpdateOf.
+    eapply (is_update_of_previous o2 o3).
+    apply H2.
+Qed.
+
+Lemma is_update_has_same_prevote_voters o1 o2
+  (is_update: IsUpdateOf o1 o2)
+  : get_prevote_voters o1 = get_prevote_voters o2.
+Proof.
+  induction is_update.
+  - auto.
+  - destruct o1.
+    destruct o2.
+    auto.
+Qed.
+
+Lemma is_update_has_same_precommit_voters o1 o2
+  (is_update: IsUpdateOf o1 o2)
+  : get_precommit_voters o1 = get_precommit_voters o2.
+Proof.
+  induction is_update.
+  - auto.
+  - destruct o1.
+    destruct o2.
+    auto.
+Qed.
+
+Lemma update_votes_with_msg_is_update_of o msg
+  : IsUpdateOf o (update_votes_with_msg o msg).
+Proof.
+  destruct o.
+  Opaque update_opaque_round_state.
+  simpl.
+  Transparent update_opaque_round_state.
+  destruct (message_to_prevote_vote msg (Round.get_prevote_voters round_state)).
+  - apply IsRoundUpdate.
+    apply SameRoundState.
+  - destruct (message_to_precommit_vote msg (Round.get_precommit_voters round_state)).
+    + apply IsRoundUpdate.
+      apply SameRoundState.
+    + apply SameRoundState.
+Qed.
+
+End IsUpdateRelation.
+
 
 Close Scope natWrapper.
 Close Scope math.
